proof/correctness/Hop1.ec
@@ -3,15 +3,48 @@ pragma Goals : printall.
 (* Hop 1: The Jasmin program is equivalent to the Jasmin program replacing the prf 
           implementation with a prf operator *)
 
-require import AllCore.
+require import AllCore List.
 
-require import XMSS_IMPL XMSS_IMPL_HOP1.
+require import RandomBytes XMSS_IMPL XMSS_IMPL_HOP1.
 
 from Jasmin require import JModel.
 
-require import Array32 Array64 Array96 Array128.
+require import Array32 Array64 Array67 Array96 Array128 Array2144.
 
-(*** AXIOMS ***)
+(*** Hash & PRF ***)
+
+lemma hash_96_hop1 (x : W8.t Array96.t) :
+    phoare [M(Syscall).__core_hash_96 : 
+      arg.`2 = x ==> res = Array32.of_list witness (Hash (to_list x))] = 1%r.
+proof.
+proc.
+admit.
+qed.
+
+lemma hash_128_hop1 (x : W8.t Array128.t) :
+    phoare [M(Syscall).__core_hash_128 : 
+      arg.`2 = x ==> res = Array32.of_list witness (Hash (to_list x))] = 1%r.
+proof.
+proc.
+admit.
+qed.
+
+lemma hash_ptr_hop1 (ptr len : W64.t) :
+    phoare [M(Syscall).__core_hash_in_ptr :
+      arg.`2=ptr /\ arg.`3=len ==> res = Hash_ptr ptr len] = 1%r.
+proof.
+proc.
+admit.
+qed.
+
+op prf_padding_bytes : W8.t list = nseq 32 (W8.of_int 3). (* 3 = XMSS_HASH_PADDING_PRF *)
+op prf_keygen_padding_bytes : W8.t list = nseq 32 (W8.of_int 4). (* 4 = XMSS_HASH_PADDING_PRF_KEYGEN *)
+
+op encode_prf (in_0  key : W8.t Array32.t) : W8.t Array96.t =
+  Array96.of_list witness (prf_padding_bytes ++ to_list in_0 ++ to_list key).
+
+op encode_prf_keygen (in_0 : W8.t Array64.t, key : W8.t Array32.t) : W8.t Array128.t =
+  Array128.of_list witness (prf_keygen_padding_bytes ++ to_list in_0 ++ to_list key).
 
 lemma prf_keygen_hop1 (out : W8.t Array32.t, _in : W8.t Array64.t, key : W8.t Array32.t) :
     phoare[M(Syscall).__prf_keygen_ : 
@@ -21,7 +54,7 @@ proof.
 proc.
 inline M(Syscall)._prf_keygen M(Syscall).__prf_keygen.
 wp ; sp.
-admit.
+idtac. admit.
 qed.
 
 lemma  prf_hop1 (out : W8.t Array32.t, _in : W8.t Array32.t, key : W8.t Array32.t):
@@ -35,97 +68,133 @@ qed.
 
 (*** STDLIB ***)
 
+lemma memset_u8_4_hop1 : 
+    equiv [M(Syscall).__memset_u8_4 ~ M_Hop1(Syscall).__memset_u8_4 : ={arg} ==> ={res}] by proc; sim.
+
+lemma memset_u8_128_hop1 : 
+    equiv [M(Syscall).__memset_u8_128 ~ M_Hop1(Syscall).__memset_u8_128 : ={arg} ==> ={res}] by proc; sim.
+
+lemma memset_u8_ptr_hop1 :
+    equiv [M(Syscall).__memset_u8_ptr ~ M_Hop1(Syscall).__memset_u8_ptr : 
+      ={arg, Glob.mem} ==> ={res,Glob.mem}].
+proof.
+proc.
+sim => />.
+qed.
+
 lemma _x_memcpy_u8u8_32_32_hop1 :
-    equiv [M(Syscall)._x_memcpy_u8u8_32_32 ~ Mp(SCall)._x_memcpy_u8u8_32_32 :
+    equiv [M(Syscall)._x_memcpy_u8u8_32_32 ~ M_Hop1(Syscall)._x_memcpy_u8u8_32_32 :
       ={arg} ==> ={res}].
 proof. proc ; inline ; sim. qed.
 
 lemma _x_memcpy_u8u8_64_64_hop1 :
-    equiv [M(Syscall)._x_memcpy_u8u8_64_64 ~ Mp(SCall)._x_memcpy_u8u8_64_64 :
+    equiv [M(Syscall)._x_memcpy_u8u8_64_64 ~ M_Hop1(Syscall)._x_memcpy_u8u8_64_64 :
       ={arg} ==> ={res}].
 proof. proc ; inline ; sim. qed.
 
 
 lemma _x_memcpy_u8u8_64_32_hop1 :
-    equiv [M(Syscall)._x_memcpy_u8u8_64_32 ~ Mp(SCall)._x_memcpy_u8u8_64_32 :
+    equiv [M(Syscall)._x_memcpy_u8u8_64_32 ~ M_Hop1(Syscall)._x_memcpy_u8u8_64_32 :
       ={arg} ==> ={res}].
 proof. proc ; inline ; sim. qed.
 
 lemma _x_memcpy_u8pu8_4_hop1 :
-    equiv [M(Syscall)._x_memcpy_u8pu8_4 ~ Mp(SCall)._x_memcpy_u8pu8_4 :
+    equiv [M(Syscall)._x_memcpy_u8pu8_4 ~ M_Hop1(Syscall)._x_memcpy_u8pu8_4 :
       ={arg,Glob.mem} ==> ={res}].
 proof. proc; inline*; sim. qed.
 
 lemma _x_memcpy_u8pu8_32_hop1 :
-    equiv [M(Syscall)._x_memcpy_u8pu8_32 ~ Mp(SCall)._x_memcpy_u8pu8_32 :
+    equiv [M(Syscall)._x_memcpy_u8pu8_32 ~ M_Hop1(Syscall)._x_memcpy_u8pu8_32 :
       ={arg,Glob.mem} ==> ={res}].
 proof. proc; inline*; sim. qed.
 
 
 lemma _x_memcpy_u8u8p_hop1 :
-    equiv [M(Syscall)._x_memcpy_u8u8p ~ Mp(SCall)._x_memcpy_u8u8p : 
+    equiv [M(Syscall)._x_memcpy_u8u8p ~ M_Hop1(Syscall)._x_memcpy_u8u8p : 
       ={arg,Glob.mem} ==> ={res}].
 proof. proc; inline*; sim => />. qed.
 
+lemma memcpy_u8u8_2_1_hop1 :
+    equiv [M(Syscall).__memcpy_u8u8_2_32_2144 ~ M_Hop1(Syscall).__memcpy_u8u8_2_32_2144 :
+      ={arg} ==> ={res}].
+proof.
+proc.
+sim => />.
+qed.
+
+lemma memcpy_u8u8_2_2_hop1 :
+    equiv [M(Syscall).__memcpy_u8u8_2_64_2144 ~ M_Hop1(Syscall).__memcpy_u8u8_2_64_2144 :
+      ={arg} ==> ={res}].
+proof.
+proc.
+sim => />.
+qed.
+
+lemma memcpy_offset_hop1 :
+    equiv[M(Syscall).__memcpy_u8u8_offset ~ M_Hop1(Syscall).__memcpy_u8u8_offset :
+       ={arg} ==> ={res}].
+proof.
+proc.
+sim => />. 
+qed.
+
 lemma ull_to_bytes_32_hop1 :
-    equiv [M(Syscall).__ull_to_bytes_32 ~ Mp(SCall).__ull_to_bytes_32 :
+    equiv [M(Syscall).__ull_to_bytes_32 ~ M_Hop1(Syscall).__ull_to_bytes_32 :
       ={arg} ==> ={res}].
 proof.
 proc ; sim => />.
 qed.
 
 lemma addr_to_bytes_hop1 :
-    equiv [M(Syscall).__addr_to_bytes ~ Mp(SCall).__addr_to_bytes : ={arg} ==> ={res}].  
+    equiv [M(Syscall).__addr_to_bytes ~ M_Hop1(Syscall).__addr_to_bytes : ={arg} ==> ={res}].  
 proof. proc ; sim => />. qed.
 
 (*** HASH ***)
 
 lemma thash_f_hop1 : 
-    equiv [M(Syscall).__thash_f ~ Mp(SCall).__thash_f : ={arg} ==> ={res}].
+    equiv [M(Syscall).__thash_f ~ M_Hop1(Syscall).__thash_f : ={arg} ==> ={res}].
 proof.
 proc.
 sp.
 seq 1 1 : (#pre /\ ={aux}); 1:call ull_to_bytes_32_hop1;auto.
-seq 1 1 : (
-   addr_as_bytes{2} = witness /\
-   bitmask{2} = witness /\
-   addr_as_bytes{1} = witness /\
-   bitmask{1} = witness /\ 
-   ={out, pub_seed, addr, aux, buf}
-); 1: auto.
-seq 1 1 : (#pre /\ ={addr}); 1:inline;auto.
-seq 1 1 : (
-   bitmask{2} = witness /\
-   bitmask{1} = witness /\ 
-   ={out, pub_seed, addr, aux, buf, addr, addr_as_bytes}
-); 1:call addr_to_bytes_hop1;auto.
-seq 1 1 : (#pre /\ ={aux}). 
-exists * (init (fun (i_0 : int) => (buf{1}.[32 + i_0])))%Array32 , addr_as_bytes{1},  pub_seed{1}.
-elim * => _P1 _P2 _P3.
-call {1} (prf_hop1 _P1 _P2 _P3).
-auto => />.
-seq 1 1 : (#pre /\ ={buf}); 1:auto.
-seq 1 1 : (#pre); 1:inline;auto.
-seq 1 1 : (#pre); 1:call addr_to_bytes_hop1;auto.
-seq 1 1 : (
-  ={out, pub_seed, addr, aux, buf, addr, addr_as_bytes, bitmask}
-).
-ecall {1} (prf_hop1 bitmask{1} addr_as_bytes{1} pub_seed{1}).
-auto.
-sp.
-seq 1 1 : (={out, buf}); last by admit.
+seq 1 1 : ( (* Same as #pre byt without the buf{1,2} = witness *)
+  addr_as_bytes{2} = witness /\
+  bitmask{2} = witness /\
+  addr_as_bytes{1} = witness /\
+  bitmask{1} = witness /\ 
+  ={out, pub_seed, addr, aux, buf}
+); 1:auto => />. 
+seq 1 1 : (#pre); 1:inline*;auto.
+seq 1 1 : ( (* Same as #pre but without addr_as_bytes{1,2} = witness *)
+  bitmask{2} = witness /\
+  bitmask{1} = witness /\ 
+  ={out, pub_seed, addr, aux, buf, addr_as_bytes}
+); 1:call addr_to_bytes_hop1;auto => />.
+seq 1 1 : (#pre). (* we already have ={aux} in #pre *)
+    + exists * (init (fun (i_0 : int) => buf{1}.[32 + i_0]))%Array32, addr_as_bytes{1}, pub_seed{1}.
+      elim * => _P1 _P2 _P3.
+      call {1} (prf_hop1 _P1 _P2 _P3); auto => />.
+seq 1 1 : (#pre) (* ={buf} is already in #pre *); 1:auto.
+seq 1 1 : (#pre). 
+    + inline M(Syscall).__set_key_and_mask M_Hop1(Syscall).__set_key_and_mask; auto.
+seq 1 1 : (#pre); 1:call addr_to_bytes_hop1;auto => />.
+seq 1 1 : (={out, pub_seed, addr, aux, buf, addr_as_bytes, bitmask}).
+    + ecall {1} (prf_hop1 bitmask{1} addr_as_bytes{1} pub_seed{1}). auto => />.
+seq 2 2 : (={buf}); last first.
+    + inline M(Syscall).__core_hash__96 M(Syscall)._core_hash_96. wp ; sp.
+      ecall {1} (hash_96_hop1 in_00{1}). auto => />.
 while (
-  ={out, pub_seed, addr, aux, buf, addr, addr_as_bytes, bitmask, i} /\
-  0 <= to_uint i{1} <= 32
-); last first.
-auto => />.
-
-admit.
-
+  #pre /\
+  0 <= to_uint i{1} <= 32 /\
+  ={i}
+).
+    + auto => /> &2 *; smt(@W64).
+    + auto => />.
 qed.
 
+
 lemma _thash_h_hop1 : 
-    equiv [M(Syscall).__thash_h ~ Mp(SCall).__thash_h : ={arg} ==> ={res}].
+    equiv [M(Syscall).__thash_h ~ M_Hop1(Syscall).__thash_h : ={arg} ==> ={res}].
 proof.
 proc.
 sp.
@@ -133,84 +202,93 @@ seq 1 1 : (={out, in_0, pub_seed, addr, buf, aux, addr_as_bytes, bitmask}); 1:ca
 seq 2 2 : (#pre); 1:inline*;auto.
 seq 1 1 : (#pre); 1:call addr_to_bytes_hop1;auto.
 seq 1 1 : (#pre). 
-  + exists * (init (fun (i_0 : int) => (buf{1}.[32 + i_0])))%Array32 , addr_as_bytes{1},  pub_seed{1}.
-elim * => _P1 _P2 _P3.
-call {1} (prf_hop1 _P1 _P2 _P3).      
+  + exists * (init (fun (i_0 : int) => (buf{1}.[32 + i_0])))%Array32, addr_as_bytes{1},  pub_seed{1}.
+    elim * => _P1 _P2 _P3. call {1} (prf_hop1 _P1 _P2 _P3). auto => />.
 seq 2 2 : (={out, in_0, pub_seed, addr, buf, aux, addr_as_bytes, bitmask}); 1:inline*;auto.
 seq 1 1 : (#pre); 1:call addr_to_bytes_hop1;auto.
 seq 1 1 : (#pre).
-  + admit. (* call to prf_hop1 *)
+  + exists * (init (fun (i_0 : int) => bitmask{1}.[0 + i_0]))%Array32, addr_as_bytes{1}, pub_seed{1}.               
+    elim * => _P1 _P2 _P3. call {1} (prf_hop1 _P1 _P2 _P3). auto => />.
 seq 1 1 : (#pre /\ ={bitmask}); 1:auto.
 seq 1 1 : (#pre); 1:inline*;auto.
 seq 1 1 : (#pre); 1:call addr_to_bytes_hop1;auto.
-seq 1 1 : (#pre); 1:admit. (* TODO: Call to  prf_hop_1 *)
+seq 1 1 : (#pre).
+  + exists * (init (fun (i_0 : int) => bitmask{1}.[32 + i_0]))%Array32, addr_as_bytes{1}, pub_seed{1}.               
+    elim * => _P1 _P2 _P3. call {1} (prf_hop1 _P1 _P2 _P3). auto => />.
 seq 1 1 : (#pre); 1:auto.
 sp.
-seq 1 1 : (={out,buf}); last by admit. (* isto isola o while. depois preciso de uma pos condicao decente para conseguir provar #post em vez de true *)
+seq 1 1 : (={buf,addr}); last first.
+  + inline M(Syscall)._core_hash_128. wp ; sp.
+      ecall {1} (hash_128_hop1 in_00{1}). auto => />.
 while (
-   ={out, in_0, pub_seed, addr, buf, aux, addr_as_bytes, bitmask, i} /\
-   0 <= to_uint i{1} <= 2 * 32 /\
-   0 <= to_uint i{2} <= 2 * 32
-); last by skip => />.
-seq 2 2 : (#pre /\ ={t}); 1:auto.
-seq 2 2 : (#pre /\ ={buf, i}).
-auto => /> *; do split; 1..4:smt(@W64). admit. admit. (*OVERFLOW*)
-skip => />. 
+  ={out, in_0, pub_seed, addr, buf, aux, addr_as_bytes, bitmask} /\ (* #pre but without i{1,2} = W64.zero *)
+  0 <= to_uint i{1} <= 2 * 32 /\
+  ={i}
+).
+    + auto => /> &2 *. smt(@W64).
+    + auto => />.
 qed.
 
 lemma hash_message_hop1 : 
-    equiv[M(Syscall).__hash_message ~ Mp(SCall).__hash_message :
+    equiv[M(Syscall).__hash_message ~ M_Hop1(Syscall).__hash_message :
         ={arg, Glob.mem} ==> ={res}].
 proof.
 proc.
 seq 2 2 : (={Glob.mem, mhash, r, root, idx, m_with_prefix_ptr, mlen, buf, buf_n}); 1:auto.
 seq 2 2 : (#pre /\ ={offset}); 1:inline*;sim => />.
-seq 10 10 : (#pre); 1:inline*;sim => />.
-admit.
+seq 10 10 : (#pre /\ ={len}); 1:inline*;sim => />.
+inline M(Syscall).__core_hash_in_ptr_ M(Syscall)._core_hash_in_ptr; wp; sp.
+ecall {1} (hash_ptr_hop1 in_ptr0{1} inlen0{1}).
+auto => />.
 qed.
 
 (*** WOTS ***)
 
 lemma expand_seed_hop1 : 
-    equiv [M(Syscall).__expand_seed ~ Mp(SCall).__expand_seed : ={arg} ==> ={res}].
+    equiv [M(Syscall).__expand_seed ~ M_Hop1(Syscall).__expand_seed : ={arg} ==> ={res}].
 proof.
 proc.
 seq 2 2 : (#pre /\ ={buf, ith_seed}); 1:auto.
-seq 2 2 : (#pre /\ ={addr}); 1:inline;auto.
+seq 2 2 : (#pre /\ ={addr}); 1:inline*;auto.
 seq 1 1 : (#pre /\ ={aux}); 1:call (_x_memcpy_u8u8_32_32_hop1);auto.
-seq 2 2 : (#pre /\ ={buf, i}); 1:auto.
+seq 1 1 : (#pre /\ ={buf}); 1:auto.
 while (
-  0 <= i{1} <= 67 /\ ={i, ith_seed, addr, outseeds, buf} /\
-  aux_list{2} = to_list aux{1}
-); last first.
-    + skip => /> &2 ; do split; 1,2,3: admit.
-    + seq 1 1 : (#pre); 1:inline*;auto.
-      seq 1 1 : (#pre /\ ={aux}).
-       * call addr_to_bytes_hop1. skip => /> &1 &2 *. admit.
-      admit.
+  0 <= i{1} <= 67 /\ 
+  ={i, ith_seed, addr, outseeds, buf}
+); last by auto => />.
+seq 1 1 : (#pre); 1:inline;auto.
+seq 1 1 : (#pre); 1:call addr_to_bytes_hop1;auto => />.
+auto => />.
+ecall {1} (prf_keygen_hop1 ith_seed{1} buf{1} inseed{1}).
+auto => /> &1 &2 *. do split.
+smt().
+smt().
+admit.
+admit.
+admit.
 qed.
 
 lemma base_w_3_2_hop1 :
-    equiv[M(Syscall).__base_w_3_2 ~ Mp(SCall).__base_w_3_2 : ={arg}  ==> ={res}].
+    equiv[M(Syscall).__base_w_3_2 ~ M_Hop1(Syscall).__base_w_3_2 : ={arg}  ==> ={res}].
 proof. proc ; sim => />. qed.
 
 lemma base_w_67_32_hop1 :
-    equiv[M(Syscall).__base_w_67_32 ~ Mp(SCall).__base_w_67_32 : ={arg}  ==> ={res}].
+    equiv[M(Syscall).__base_w_67_32 ~ M_Hop1(Syscall).__base_w_67_32 : ={arg}  ==> ={res}].
 proof. proc ; sim => />. qed.
 
 lemma csum_hop1 :
-    equiv[M(Syscall).__csum ~ Mp(SCall).__csum : ={arg} ==> ={res}].
+    equiv[M(Syscall).__csum ~ M_Hop1(Syscall).__csum : ={arg} ==> ={res}].
 proof. proc ; sim => />. qed. 
 
 lemma checksum_hop1 :
-    equiv[M(Syscall).__wots_checksum ~ Mp(SCall).__wots_checksum : ={arg} ==> ={res}].
+    equiv[M(Syscall).__wots_checksum ~ M_Hop1(Syscall).__wots_checksum : ={arg} ==> ={res}].
 proof.
 proc.
 sim => />.
 qed.
 
 lemma chain_lengths_hop1 :
-    equiv [M(Syscall).__chain_lengths ~ Mp(SCall).__chain_lengths : ={arg} ==> ={res}].
+    equiv [M(Syscall).__chain_lengths ~ M_Hop1(Syscall).__chain_lengths : ={arg} ==> ={res}].
 proof.
 proc.
 seq 1 1 : (#pre /\ ={t}); 1:auto.
@@ -219,120 +297,231 @@ seq 1 1 : (#pre); 1:auto.
 seq 1 1 : (#pre); 1:call checksum_hop1;auto.
 qed.
 
-lemma gen_chain_hop1 :
-    equiv [M(Syscall).__gen_chain ~ Mp(SCall).__gen_chain : ={arg,Glob.mem} ==> ={res}].
-proof.
-proc.
-seq 1 1 : (={out, in_ptr, start, steps, pub_seed, addr}); 1:call _x_memcpy_u8u8p_hop1;auto.
-seq 3 3 : (#pre /\ ={t}); 1:auto.
-admit.
-qed.
-
 lemma gen_chain_inplace_hop1 :
-    equiv [M(Syscall).__gen_chain_inplace ~ Mp(SCall).__gen_chain_inplace :
-      ={arg} ==> ={res}].
+    equiv [M(Syscall).__gen_chain_inplace_ ~ M_Hop1(Syscall).__gen_chain_inplace_ : ={arg} ==> ={res}].
 proof.
-proc.
-sp.
-while (={i,out,pub_seed,addr,steps}); last by skip => />.
-seq 1 1 : (#pre); 1:inline;auto.
-call _thash_f_hop1;auto => />. 
+proc ; auto => />.
+inline M(Syscall)._gen_chain_inplace M_Hop1(Syscall)._gen_chain_inplace.
+inline M(Syscall).__gen_chain_inplace  M_Hop1(Syscall).__gen_chain_inplace.
+seq 15 15 : (#pre /\ ={start1, start0, addr0, addr1, steps0, steps1, out0, out1, pub_seed0, pub_seed1}); 1:auto => />.
+wp; sp.
+while (
+  ={out, start, steps, pub_seed, addr, i, t, start1, steps1, out0, out1, addr1, pub_seed1, pub_seed0}
+); last first.
+    + auto => />.
+    + auto => />. seq 1 1 : (#pre); 1:inline;auto=>/>.
+      inline M(Syscall).__thash_f_ M_Hop1(Syscall).__thash_f_.
+      inline M(Syscall)._thash_f M_Hop1(Syscall)._thash_f. wp;sp.
+      call thash_f_hop1; auto => />.      
 qed.
 
-lemma _gen_chain_inplace_hop1 :
-    equiv [M(Syscall).__gen_chain_inplace_ ~ Mp(SCall).__gen_chain_inplace_ :
-      ={arg} ==> ={res}].
+
+lemma gen_chain_inplace_2_hop1 :
+    equiv [M(Syscall).__gen_chain_inplace_ ~ M_Hop1(Syscall).__gen_chain_inplace_ : ={arg} ==> ={res}].
 proof.
-proc.
-inline M(Syscall)._gen_chain_inplace Mp(SCall)._gen_chain_inplace.
-sp; wp.
-call gen_chain_inplace_hop1 ; auto.
+proc ; auto => />.
+inline M(Syscall)._gen_chain_inplace M_Hop1(Syscall)._gen_chain_inplace.
+inline M(Syscall).__gen_chain_inplace  M_Hop1(Syscall).__gen_chain_inplace.
+seq 15 15 : (#pre /\ ={start1, start0, addr0, addr1, steps0, steps1, out0, out1, pub_seed0, pub_seed1}); 1:auto => />.
+wp; sp.
+while (
+  ={out, start, steps, pub_seed, addr, i, t, start1, steps1, out0, out1, addr1, pub_seed1, pub_seed0}
+); last first.
+    + auto => />.
+    + auto => />. seq 1 1 : (#pre); 1:inline;auto=>/>.
+      inline M(Syscall).__thash_f_ M_Hop1(Syscall).__thash_f_.
+      inline M(Syscall)._thash_f M_Hop1(Syscall)._thash_f. wp;sp.
+      call thash_f_hop1; auto => />.      
 qed.
 
 lemma wots_pkgen_hop1 :
-    equiv [M(Syscall).__wots_pkgen ~ Mp(SCall).__wots_pkgen : ={arg} ==> ={res}].
+    equiv [M(Syscall).__wots_pkgen ~ M_Hop1(Syscall).__wots_pkgen : ={arg} ==> ={res}].
 proof.
 proc.
 seq 1 1 : (#pre /\ ={pk, addr}).
-  + inline M(Syscall).__expand_seed_ M(Syscall)._expand_seed Mp(SCall).__expand_seed_  Mp(SCall)._expand_seed. wp ; sp. call expand_seed_hop1. auto.
+  + inline M(Syscall).__expand_seed_ M(Syscall)._expand_seed M_Hop1(Syscall).__expand_seed_  M_Hop1(Syscall)._expand_seed. wp ; sp. call expand_seed_hop1. auto.
 sp. 
 while (={i,pk,pub_seed,addr} /\ 0 <= i{1} <= 67); last by auto.
 seq 1 1 : (#pre /\ ={chain}); 1:auto.
 seq 1 1 : (#pre); 1:inline;auto.
-call _gen_chain_inplace_hop1.
+call {1} (gen_chain_inplace_hop1).
 auto => /> /#.
 qed.
 
 lemma wots_sign_hop1 :
-    equiv [M(Syscall).__wots_sign ~ Mp(SCall).__wots_sign : ={arg} ==> ={res}].
+    equiv [M(Syscall).__wots_sign ~ M_Hop1(Syscall).__wots_sign : ={arg} ==> ={res}].
 proof.
 proc.
-sp.
-seq 1 1 : (={sig, msg, seed, pub_seed, addr, lengths}).
+seq 2 2 : (={sig, msg, seed, pub_seed, addr, lengths}).
   + inline M(Syscall).__chain_lengths_ M(Syscall)._chain_lengths 
-           Mp(SCall).__chain_lengths_ Mp(SCall)._chain_lengths; wp ; sp.
-    call chain_lengths_hop1. auto.
+           M_Hop1(Syscall).__chain_lengths_ M_Hop1(Syscall)._chain_lengths; wp ; sp.
+    call chain_lengths_hop1. auto => />.
 seq 1 1 : (#pre). 
   + inline M(Syscall).__expand_seed_ M(Syscall)._expand_seed
-           Mp(SCall).__expand_seed_ Mp(SCall)._expand_seed; wp ; sp.
+           M_Hop1(Syscall).__expand_seed_ M_Hop1(Syscall)._expand_seed; wp ; sp.
     call expand_seed_hop1. auto.
 sp.
 while (={sig, msg, seed, pub_seed, addr, lengths, i} /\ 0 <= i{1} <= 67); last by skip => />.
-seq 1 1 : (#pre /\ ={chain}); 1:auto.
-seq 1 1 : (#pre /\ ={addr}); 1:inline;auto.
-seq 1 1 : (#pre /\ ={aux_0, aux_1}); 1:call gen_chain_inplace_hop1;auto.
-(* TODO: call the gen_chain locla function in the code (not the inline) *)
+seq 2 2 : (#pre /\ ={chain,addr}); 1:inline;auto.
+seq 1 1 : (#pre /\ ={aux_0, aux_1}); 1:call {1} (gen_chain_inplace_hop1);auto => />. 
 auto => /> /#.
 qed.
 
 lemma wots_pk_from_sig_hop1 :
-    equiv [M(Syscall).__wots_pk_from_sig ~ Mp(SCall).__wots_pk_from_sig : 
+    equiv [M(Syscall).__wots_pk_from_sig ~ M_Hop1(Syscall).__wots_pk_from_sig : 
       ={arg,Glob.mem} ==> ={res}].
 proof.
 proc.
 sp.
 seq 1 1 : (={pk, sig_ptr, msg, pub_seed, addr, lengths, Glob.mem}).
   + inline M(Syscall).__chain_lengths_ M(Syscall)._chain_lengths
-           Mp(SCall).__chain_lengths_ Mp(SCall)._chain_lengths; wp ; sp.
-    call chain_lengths_hop1. auto.
+           M_Hop1(Syscall).__chain_lengths_ M_Hop1(Syscall)._chain_lengths; wp ; sp.
+    call chain_lengths_hop1. auto => />.
 sp.
-while (={pk, sig_ptr, msg, pub_seed, addr, lengths, i, Glob.mem} /\ 0 <= i{1} <= 67); last by skip => />.
+while (={pk, sig_ptr, msg, pub_seed, addr, lengths, i, Glob.mem} /\ 0 <= i{1} <= 67); last by skip => />. 
 seq 1 1 : (#pre /\ ={chain}); 1:auto.
 seq 1 1 : (#pre /\ ={addr}); 1:inline*;auto.
 seq 3 3 : (#pre /\ ={start,steps}); 1:auto.
 seq 2 2 : (#pre /\ ={t}); 1:auto.
-seq 1 1 : (#pre /\ ={aux_0, aux_1}).
-  + inline M(Syscall).__gen_chain_ M(Syscall)._gen_chain
-           Mp(SCall).__gen_chain_ Mp(SCall)._gen_chain ; wp ; sp.
-    call gen_chain_hop1. skip => />. 
-skip => /> /#.
+seq 1 1 : (#pre /\ ={aux_0}).
+  + call _x_memcpy_u8u8p_hop1. auto => /> .
+seq 1 1 : (#pre); 1:auto => />.
+auto => />. (* Simplify #post *)
+seq 1 1 : (#pre /\ ={aux_1}).
+  + call gen_chain_inplace_hop1; auto => />.
+auto => /> /#.
 qed.
 
 (*** XMSS COMMONS ***)
 
 lemma ltree_hop1 :
-    equiv [M(Syscall).__l_tree ~ Mp(SCall).__l_tree :
-      ={arg,Glob.mem} ==> ={res}].
+    equiv [M(Syscall).__l_tree ~ M_Hop1(Syscall).__l_tree :
+      ={arg, Glob.mem} ==> ={res, Glob.mem}].
 proof.
 proc.
-sp.
-seq 1 1 : (#pre /\ ={addr}); 1:inline;auto.
-admit.
+wp; sp.
+seq 1 1 : (#pre).
+  + inline;auto.
+seq 1 1 : (#post);last first. (* isto isola o while [que vai ser o segundo subgoal] *)
+  + call _x_memcpy_u8u8_32_32_hop1; auto =>/>.
+while (
+  ={buf0, buf1, l, height, leaf, wots_pk, pub_seed, addr, Glob.mem}
+); last first.
+    + skip => /> *. 
+    + seq 2 2 : (#pre /\ ={parent_nodes}); 1:auto.
+      seq 2 2 : (={buf0, buf1, l, height, leaf, wots_pk, pub_seed, addr, Glob.mem}). (* Isto isola o primeiro while *)
+        * while (#pre /\ ={i}); last by auto => />.
+          seq 1 1 : (#pre /\ ={tree_index}); 1:auto=>/>.
+          seq 1 1 : (#pre); 1:inline;auto=>/>.
+          seq 2 2 : (#pre /\ ={offset_in, bytes}); 1:auto=>/>.
+          seq 1 1 : (#pre /\ ={buf0}); 1:call memcpy_u8u8_2_1_hop1; auto => />.
+          seq 3 3 : (#pre /\ ={bytes}); 1:auto => />.
+          seq 1 1 : (#pre /\ ={buf1}); 1:call memcpy_u8u8_2_2_hop1; auto => />.
+          seq 1 1 : (#pre); 1:call _thash_h_hop1; auto => />.
+          seq 1 1 : (#pre /\ ={offset_out}); 1:auto => />.
+          call memcpy_offset_hop1. auto => />.
+        * seq 2 2 : (#pre /\ ={t}); 1:auto=> />.
+          if; first by auto => />.
+              (* first subgoal of if *)
+              - seq 6 6 : (#pre /\ ={offset_out, offset_in}); 1:auto=> />.
+                seq 2 2 : (#pre). (* isto isola o while *)
+                    * while (={j, wots_pk, offset_in, offset_out}); last by auto => />. auto => />.
+                    * seq 3 3 : (#pre); 1:auto => />.
+                      inline; auto => />.
+              (* second subgoal of if *) 
+              - seq 2 2 : (#pre); 1: auto => /> *. 
+                inline ; auto => />.
 qed.
 
 lemma compute_root_hop1 :
-  equiv [M(Syscall).__compute_root ~ Mp(SCall).__compute_root :
+  equiv [M(Syscall).__compute_root ~ M_Hop1(Syscall).__compute_root :
       ={arg,Glob.mem} ==> ={res}].
 proof.
 proc.
-sp.
+(*
+seq 5 5 : (={root, leaf, leaf_idx, _auth_path_ptr, pub_seed, addr, buffer, thash_in, auth_path_ptr, t32, Glob.mem}).
+  + auto.
 if; first by auto.
-  + admit.
-  + admit.
+  + seq 1 1 : (#pre /\ ={aux}); 1:call _x_memcpy_u8u8_32_32_hop1; auto => />.
+    seq 1 1 : (#pre); 1:auto => />.
+    seq 1 1 : (#pre); 1:call _x_memcpy_u8u8p_hop1; auto => />.
+    seq 2 2 : (#pre); 1:auto => />.
+    seq 1 1 : (#pre /\ ={i}); 1:auto.
+    seq 1 1 : (#pre /\ ={i}); 1:auto. (* isolates the while loop *)
+      * while ( (* This subgoal corresponds to the while loop *)
+          #pre
+        ).
+          (* first subgoal of while *)
+          + seq 1 1 : (#pre /\ ={tree_height}); 1:auto.
+            seq 3 3 : (#pre); 1:inline;auto=> />.
+            seq 3 3 : (#pre). (* isolates the if *)
+                - seq 2 2 : (={root, leaf, leaf_idx, _auth_path_ptr, pub_seed, addr, buffer, 
+                               thash_in, auth_path_ptr, t32, Glob.mem, t32, aux, i, tree_height} /\
+                               (i{1} \ult (of_int 9)%W64) /\ (i{2} \ult (of_int 9)%W64)); 1:auto => />.
+                  if; 1:auto => />.
+                     (* First subgoal of if *)
+                     * seq 1 1 : (#pre); 1:auto => />.
+                       seq 1 1 : (#pre /\ ={aux, aux_0}); 1:call _thash_h_hop1; auto => />.
+                       seq 2 2 : (#pre); 1:auto => />.
+                       call _x_memcpy_u8u8p_hop1. auto => />.
+                     (* Second subgoal of if : We have that t32 = W32.zero*)
+                     * seq 1 1 : (#pre /\ t32{1}=W32.zero); 1:auto => />.
+                       seq 1 1 : (#pre /\ ={aux, aux_0}).
+                          - call _thash_h_hop1; auto => />.
+                       seq 2 2 : (#pre); 1:auto => />.
+                       seq 1 1 : (#pre); 1:call _x_memcpy_u8u8p_hop1; auto => />.
+                       auto => /> &1 &2 *.  admit. (* FIXME *)
+                - skip => />.
+          (* last subgoal of while *)
+          + skip => />.
+      * seq 1 1 : (#pre); 1:inline;auto => />.
+        seq 1 1 : (#pre); 1:auto.
+        seq 1 1 : (#pre); 1:inline;auto=>/>.
+        call _thash_h_hop1. auto => />.      
+  + seq 1 1 : (#pre); 1:call _x_memcpy_u8u8_64_32_hop1; auto => />.
+    seq 1 1 : (#pre /\ ={aux}); 1:call _x_memcpy_u8u8p_hop1; auto => />.
+    seq 1 1 : (#pre); 1:auto => />.
+    seq 1 1 : (#pre /\ ={auth_path_ptr}); 1:auto => />.
+    seq 1 1 : (#pre /\ ={i}); 1:auto.
+    seq 1 1 : (#pre). (* isolates the while loop *)
+      * while ( (* This subgoal corresponds to the while loop *)
+          #pre
+        ).
+          (* first subgoal of while *)
+          + seq 1 1 : (#pre /\ ={tree_height}); 1:auto.
+            seq 3 3 : (#pre); 1:inline;auto=> />.
+            seq 3 3 : (#pre). (* isolates the if *)
+                - seq 2 2 : (={root, leaf, leaf_idx, _auth_path_ptr, pub_seed, addr, buffer, 
+                               thash_in, auth_path_ptr, t32, Glob.mem, t32, aux, i, tree_height} /\
+                               (i{1} \ult (of_int 9)%W64) /\ (i{2} \ult (of_int 9)%W64)); 1:auto => />.
+                  if; 1:auto => />.
+                     (* First subgoal of if *)
+                     * seq 1 1 : (#pre); 1:auto => />.
+                       seq 1 1 : (#pre /\ ={aux, aux_0}).
+                           + call _thash_h_hop1; auto => />.
+                       seq 2 2 : (#pre); 1:auto => />.
+                       seq 1 1 : (#pre). 
+                           + call _x_memcpy_u8u8p_hop1. auto => />.
+                       auto => /> *. admit.
+                     (* Second subgoal of if : We have that t32 = W32.zero*)
+                     * seq 1 1 : (#pre /\ t32{1}=W32.zero); 1:auto => />.
+                       seq 1 1 : (#pre /\ ={aux, aux_0}).
+                          - call _thash_h_hop1; auto => />.
+                       seq 2 2 : (#pre); 1:auto => />.
+                       seq 1 1 : (#pre); 1:call _x_memcpy_u8u8p_hop1; auto => />.
+                       auto => /> &1 &2 *.  admit. (* FIXME *)
+                - skip => />.
+          (* last subgoal of while *)
+          + skip => />.
+      * admit. (* This subgoal corresponds to the while loop *)
+      * seq 1 1 : (#pre); 1:inline;auto => />.
+        seq 1 1 : (#pre); 1:auto.
+        seq 1 1 : (#pre); 1:inline;auto=>/>.
+        call _thash_h_hop1. auto => />.
 qed.
 
 lemma gen_leaf_wots_hop1 :
-    equiv[M(Syscall).__gen_leaf_wots ~ Mp(SCall).__gen_leaf_wots :
+    equiv[M(Syscall).__gen_leaf_wots ~ M_Hop1(Syscall).__gen_leaf_wots :
       ={arg,Glob.mem} ==> ={res}].
 proof.
 proc.
@@ -340,19 +529,21 @@ seq 2 2 : (={Glob.mem, leaf, sk_seed, pub_seed, ltree_addr, ots_addr, pk, _0}); 
 seq 1 1 : (#pre /\ ={pk}); 1:call wots_pkgen_hop1;auto. 
 seq 1 1 : (#pre).
   + inline M(Syscall).__l_tree_ M(Syscall)._l_tree
-           Mp(SCall).__l_tree_ Mp(SCall)._l_tree. wp ; sp.
+           M_Hop1(Syscall).__l_tree_ M_Hop1(Syscall)._l_tree. wp ; sp.
     call ltree_hop1;auto.
 auto.
+*)
+admit.
 qed.
 
 lemma set_result_hop1 : 
-    equiv [M(Syscall).__set_result ~ Mp(SCall).__set_result :
+    equiv [M(Syscall).__set_result ~ M_Hop1(Syscall).__set_result :
       ={arg,Glob.mem} ==> ={res}].
 proof. proc ; sim => />. qed.
 
 lemma xmssmt_core_sign_open :
-    equiv [M(Syscall).__xmssmt_core_sign_open ~ Mp(SCall).__xmssmt_core_sign_open :
-      ={arg,Glob.mem} ==> ={res}].
+    equiv [M(Syscall).__xmssmt_core_sign_open ~ M_Hop1(Syscall).__xmssmt_core_sign_open :
+      ={arg, Glob.mem} ==> ={res, Glob.mem}].
 proof.
 proc.
 seq 13 13 : (={buf, leaf, ltree_addr, node_addr, root, wots_pk, sm_offset, pub_root,
@@ -363,7 +554,8 @@ seq 7 7 : (#pre /\ ={offset_out, offset_in, bytes}); 1:inline*;sim => />.
 seq 1 1 : (#pre); 1:call _x_memcpy_u8u8p_hop1;auto.
 seq 4 4 : (#pre /\ ={idx_hash}); 1:auto.
 seq 1 1 : (#pre).
-  + call hash_message_hop1. skip => /> *. admit.
+  + call hash_message_hop1. skip => /> *.   
+admit.
 seq 3 3 : (#pre /\ ={sm_offset, i}); 1:auto.
 admit.
 qed.
@@ -372,7 +564,7 @@ qed.
 
 (* TODO: Remove the _array suffix *)
 lemma treehash_array_hop1 :
-    equiv[M(Syscall).__treehash_array ~ Mp(SCall).__treehash_array : 
+    equiv[M(Syscall).__treehash_array ~ M_Hop1(Syscall).__treehash_array : 
         ={Glob.mem, arg} ==> ={res}].
 proof.
 proc.
@@ -387,7 +579,7 @@ admit.
 qed.
 
 lemma xmssmt_core_seed_keypair_hop1 :
-    equiv[M(Syscall).__xmssmt_core_seed_keypair ~ Mp(SCall).__xmssmt_core_seed_keypair :
+    equiv[M(Syscall).__xmssmt_core_seed_keypair ~ M_Hop1(Syscall).__xmssmt_core_seed_keypair :
       ={Glob.mem, arg} ==> ={res}].
 proof.
 proc.
@@ -400,14 +592,14 @@ seq 1 1 : (#pre /\ ={aux_1}); 1:inline*;sim.
 seq 1 1 : (#pre); 1:auto.
 seq 2 2 : (#pre /\ ={aux_1}); 1:inline*;sim.
 inline M(Syscall).__treehash_array_ M(Syscall)._treehash_array
-       Mp(SCall).__treehash_array_ Mp(SCall)._treehash_array.
+       M_Hop1(Syscall).__treehash_array_ M_Hop1(Syscall)._treehash_array.
 wp ; sp.
 call treehash_array_hop1.
 skip => />.
 qed.
 
 lemma xmssmt_core_keypair_hop1 :
-    equiv[M(Syscall).__xmssmt_core_keypair ~ Mp(SCall).__xmssmt_core_keypair :
+    equiv[M(Syscall).__xmssmt_core_keypair ~ M_Hop1(Syscall).__xmssmt_core_keypair :
       ={arg,Glob.mem} ==> ={res}].
 proof.
 proc.
@@ -418,7 +610,7 @@ skip => />.
 qed.
 
 lemma xmssmt_core_sign_hop1 :
-    equiv [M(Syscall).__xmssmt_core_sign ~ Mp(SCall).__xmssmt_core_sign :
+    equiv [M(Syscall).__xmssmt_core_sign ~ M_Hop1(Syscall).__xmssmt_core_sign :
       ={Glob.mem, arg} ==> ={res}].
 proof.
 proc.
@@ -426,28 +618,38 @@ seq 10 10 : (={Glob.mem, sk, sm_ptr, smlen_ptr, m_ptr, mlen, auth_path, buf, idx
                ots_addr, pub_root, pub_seed, root, sig, sk_prf, sk_seed}); 1:sim.
 seq 3 3 : (#pre); 1:inline*;sim.
 seq 4 4 : (#pre /\ ={idx}); 1:sim.
-if; first by auto.
-  + admit.
-  + admit.
+if; first by auto. 
+(* First subgoal of first if *)
+  + seq 1 1 : (#pre /\ ={aux}); 1:call memset_u8_4_hop1; auto.
+    seq 1 1 : (#pre); 1:auto.
+    seq 1 1 : (#pre /\ ={aux_0}); 1:call memset_u8_128_hop1; auto.
+    seq 1 1 : (#pre); 1:auto. 
+    if; first by auto => />.
+    * admit. (* First subgoal of the second if *) 
+    * admit. (* Second subgoal of the second if *)
+(* Last subgoal of the first if *)
+  + if. auto => /> &1 &2 *. admit.
+    * admit.
+    * auto => /> &2. admit.
 qed.
 
 (*** XMSS ***)
 
 lemma xmss_keypair_hop1 :
-    equiv[M(Syscall).__xmss_keypair ~ Mp(SCall).__xmss_keypair :
+    equiv[M(Syscall).__xmss_keypair ~ M_Hop1(Syscall).__xmss_keypair :
       ={arg,Glob.mem} ==> ={res}].
 proof.
 proc.
 seq 4 4 : (={Glob.mem, pk, sk, oid}); 1:auto.
 seq 1 1 : (#pre /\ ={aux, aux_0}).
   + inline M(Syscall).__xmssmt_core_keypair_ M(Syscall)._xmssmt_core_keypair
-           Mp(SCall).__xmssmt_core_keypair_ Mp(SCall)._xmssmt_core_keypair.
+           M_Hop1(Syscall).__xmssmt_core_keypair_ M_Hop1(Syscall)._xmssmt_core_keypair.
     wp ; sp. call xmssmt_core_keypair_hop1. skip => />.
 sim.
 qed.
 
 lemma xmss_sign_hop1 :
-    equiv[M(Syscall).__xmss_sign ~ Mp(SCall).__xmss_sign :
+    equiv[M(Syscall).__xmss_sign ~ M_Hop1(Syscall).__xmss_sign :
       ={arg, Glob.mem} ==> ={res}].
 proof.
 proc.
